[wip]

Clear/EVMState.lean
@@ -414,61 +414,50 @@ instance : Inhabited EVMState :=
 
 abbrev EVM := EVMState
 
-def preserved : EVMState → EVMState → Prop :=
-  (Eq on EVMState.account_map) ∩
-  (Eq on EVMState.hash_collision) ∩
-  (Eq on EVMState.execution_env)
+instance instPreorderFinmap : Preorder (Finmap (λ _ : List UInt256 ↦ UInt256)) where
+  le a b := a.keys ⊆ b.keys ∧ ∀ {key}, key ∈ a → a.lookup key = b.lookup key
+  le_refl := by aesop
+  le_trans := by aesop (add safe forward subset_trans)
 
-def preserves_account_map :
-  {evm evm' : EVMState} → preserved evm evm' → evm.account_map = evm'.account_map := by
-  intro evm evm' h
-  exact h.1.1
+structure Preserved (a : EVMState) (b : EVMState) : Prop where
+  account_map : (Eq on EVMState.account_map) a b
+  hash_collision : (Eq on EVMState.hash_collision) a b
+  execution_env : (Eq on EVMState.execution_env) a b
+  keccak_map : a.keccak_map ≤ b.keccak_map
 
-def preserves_collision :
-  {evm evm' : EVMState} → preserved evm evm' → evm.hash_collision = evm'.hash_collision := by
-  intro _ _ h
-  exact h.1.2
-
-def preserves_execution_env :
-  {evm evm' : EVMState} → preserved evm evm' → evm.execution_env = evm'.execution_env := by
-  intro _ _ h
-  exact h.2
-
-lemma preserved_def {e₀ e₁ : EVM} : preserved e₀ e₁ =
-  (e₀.account_map = e₁.account_map ∧
-  e₀.hash_collision = e₁.hash_collision ∧
-  e₀.execution_env = e₁.execution_env) := by
-  unfold preserved
-  dsimp [(· ∩ ·)]
-  simp [Function.onFun, and_assoc]
-
-@[simp]
-lemma preserved_rfl {e : EVM} : preserved e e := by
-  unfold preserved
-  dsimp [(· ∩ ·)]
-  simp
-
-lemma preserved_symm {e₀ e₁ : EVM} : preserved e₀ e₁ = preserved e₁ e₀ := by
-  rw [preserved_def, preserved_def]
+lemma Preserved_def {σ₀ σ₁ : EVM} : Preserved σ₀ σ₁ =
+  (σ₀.account_map    = σ₁.account_map ∧
+   σ₀.hash_collision = σ₁.hash_collision ∧
+   σ₀.execution_env  = σ₁.execution_env ∧
+   σ₀.keccak_map     ≤ σ₁.keccak_map) := by
   ext
-  apply Iff.intro <;> {
-    intro ⟨acc, col, env⟩
-    symm at acc col env
-    exact ⟨acc, col, env⟩
-  }
+  apply Iff.intro
+  intro h
+  obtain ⟨_,_,_,_⟩ := h
+  all_goals tauto
+
+namespace Preserved
 
 @[simp]
-lemma preserved_trans {e₀ e₁ e₂ : EVM} :
-  preserved e₀ e₁ → preserved e₁ e₂ → preserved e₀ e₂ := by
-  unfold preserved
-  dsimp [(· ∩ ·)]
+lemma refl {e : EVM} : Preserved e e := by
+  constructor
+  all_goals simp
+
+lemma trans {e₀ e₁ e₂ : EVM} :
+  Preserved e₀ e₁ → Preserved e₁ e₂ → Preserved e₀ e₂ := by
   intro h₀ h₁
-  have acc := Eq.trans (preserves_account_map h₀) (preserves_account_map h₁)
-  have col := Eq.trans (preserves_collision h₀) (preserves_collision h₁)
-  have env := Eq.trans (preserves_execution_env h₀) (preserves_execution_env h₁)
-  apply And.intro
-  apply And.intro
-  all_goals assumption
+  have acc := Eq.trans h₀.account_map h₁.account_map
+  have col := Eq.trans h₀.hash_collision h₁.hash_collision
+  have env := Eq.trans h₀.execution_env h₁.execution_env
+  have kec := le_trans h₀.keccak_map h₁.keccak_map
+  constructor <;> assumption
+
+end Preserved
+
+instance instPreorderEVMState : Preorder EVMState where
+  le := Preserved
+  le_refl := @Preserved.refl
+  le_trans := @Preserved.trans
 
 -- functions for querying balance
 
@@ -662,16 +651,16 @@ def evm_return (σ : EVMState) (mstart s : UInt256) : EVMState :=
 def evm_revert (σ : EVMState) (mstart s : UInt256) : EVMState :=
   σ.evm_return mstart s
 
-lemma mstore_preserves {evm} {pos val} : preserved evm (evm.mstore pos val) := by
+lemma mstore_preserved {σ} {pos val} : Preserved σ (σ.mstore pos val) := by
   unfold mstore updateMemory
-  rw [preserved_def]
+  rw [Preserved_def]
   simp
 
-lemma sload_eq_of_preserved {σ₀ σ₁} {pos} (h : preserved σ₀ σ₁) :
+lemma sload_eq_of_preserved {σ₀ σ₁} {pos} (h : Preserved σ₀ σ₁) :
   sload σ₀ pos = sload σ₁ pos := by
   unfold sload lookupAccount
-  rw [ preserves_account_map h
-     , preserves_execution_env h
+  rw [ h.account_map
+     , h.execution_env
      ]
 
 end
