Generated/erc20shim/ERC20Shim/Predicate.lean
@@ -17,6 +17,11 @@ structure ERC20 where
   balances : BalanceMap
   allowances : AllowanceMap
 
+def acc (a : Option UInt256) : Prop :=
+  match a with
+  | some el => el ∉ ERC20Private.toFinset
+  | none => true
+
 structure IsERC20 (erc20 : ERC20) (s : State) : Prop where
   hasSupply : s.evm.sload ERC20Private.totalSupply = erc20.supply
 
@@ -24,9 +29,6 @@ structure IsERC20 (erc20 : ERC20) (s : State) : Prop where
     ∀ {account}, (account ∈ erc20.balances) →
     ∃ (address : UInt256),
     s.evm.keccak_map.lookup [ ↑account , ERC20Private.balances ] = some address ∧
-
-    -- address ∈ s.evm.keccak_map.lookup [ ↑account , ERC20Private.balances ]
-
     erc20.balances.lookup account = some (s.evm.sload address)
 
   hasAllowance :
@@ -36,8 +38,9 @@ structure IsERC20 (erc20 : ERC20) (s : State) : Prop where
     s.evm.keccak_map.lookup [ ↑spender , intermediate ] = some address →
     erc20.allowances.lookup ⟨owner, spender⟩ = some (s.evm.sload address)
 
+  -- mem : account ∉ erc20.balances
   storageDom :
-    (storage s.evm).keys =
+    s.evm.storage.keys =
       { address | ∃ account,
         account ∈ erc20.balances ∧
         some address = s.evm.keccak_map.lookup [ ↑account, ERC20Private.balances ] } ∪
@@ -46,6 +49,12 @@ structure IsERC20 (erc20 : ERC20) (s : State) : Prop where
         ∃ intermediate, s.evm.keccak_map.lookup [ ↑owner , ERC20Private.allowances ] = some intermediate ∧
         s.evm.keccak_map.lookup [ ↑spender , intermediate ] = some address } ∪
       ERC20Private.toFinset
+
+  block_acc_range :
+    ∀ {account}, acc (s.evm.keccak_map.lookup [ ↑account, ERC20Private.balances ])
+
+  -- block_allowance_range :
+  --   ∀ {owner}, s.evm.keccak_map.lookup [ ↑owner, ERC20Private.allowances ] ∉ ERC20Private.toFinset
 
     -- equivalent statements
     -- s.evm.sload address ∈ erc20.balances.lookup account
@@ -70,12 +79,21 @@ lemma IsERC20_of_ok_forall_store {erc20} {evm} {s₀ s₁} :
   · have := get_evm_of_ok ▸ is_erc.storageDom
     exact this
 
-lemma IsERC20_of_ok_of_preserved {erc20} {store} {σ₀ σ₁} (h : preserved σ₀ σ₁) : 
+lemma IsERC20_of_ok_of_Preserved {erc20} {store} {σ₀ σ₁} (h : Preserved σ₀ σ₁) : 
   IsERC20 erc20 (Ok σ₀ store) → IsERC20 erc20 (Ok σ₁ store) := by
   sorry
   
 lemma IsERC20_of_preservesEvm {erc20} {s₀ s₁} :
   preservesEvm s₀ s₁ → IsERC20 erc20 s₀ → IsERC20 erc20 s₁ := by
+  sorry
+
+lemma sload_of_IsERC20_outside {erc20} {s} (h : IsERC20 erc20 s) :
+  ∀ {addr}, addr ∉ s.evm.storage.keys → s.evm.sload addr = 0 := by
+  sorry
+
+lemma t {erc20} {s₀ s₁} (is_erc20 : IsERC20 erc20 s₀) (h : preservesEvm s₀ s₁) :
+  ∀ {addr}, addr ∉ s₀.evm.keccak_range ∧ addr ∈ s₁.evm.keccak_range →
+  addr ∉ s₀.evm.storage.keys := by
   sorry
 
 end Generated.erc20shim.ERC20Shim
