Generated/erc20shim/ERC20Shim/fun_balanceOf_user.lean
@@ -25,38 +25,57 @@ lemma fun_balanceOf_abs_of_concrete {s₀ s₉ : State} {var var_account} :
   rcases s₀ with ⟨evm, varstore⟩ | _ | _ <;> [simp only; aesop_spec; aesop_spec]
   apply spec_eq
   clr_funargs
-  intro hasFuel ⟨s, keccak, code⟩ erc20 is_erc20
+  intro hasFuel ⟨s, mapping, code⟩ erc20 is_erc20
 
   clr_varstore
 
-  unfold A_mapping_index_access_mapping_address_uint256_of_address at keccak
-  simp at keccak
-  clr_spec at keccak
+  -- what we can get right now from mapping function
+  unfold A_mapping_index_access_mapping_address_uint256_of_address at mapping
+  simp at mapping
+  clr_spec at mapping
+  obtain ⟨preservesEvm, s_isOk, keccak⟩ := mapping  
+  obtain ⟨evmₛ, varstoreₛ, s_eq_ok⟩ := State_of_isOk s_isOk
 
-  have : Address.ofUInt256 var_account ∈ erc20.balances := sorry
-  obtain ⟨address, hasAddress, hasBalance⟩ := is_erc20.hasBalance this
-  obtain ⟨preserves, is_ok, lookup⟩ := keccak hasAddress
-  obtain ⟨evmₛ, varstoreₛ, ok_state⟩ := State_of_isOk is_ok
-
+  -- simplify contract
   unfold reviveJump at code
-  simp [ok_state] at code lookup
-
-  rw [ ← State.insert_of_ok,  ← State.insert_of_ok, lookup ] at code
+  simp [s_eq_ok] at code
+  rw [ ← State.insert_of_ok,  ← State.insert_of_ok, ← s_eq_ok ] at code
   clr_varstore
 
-  have preserves_final : preservesEvm (Ok evm varstore) (Ok evmₛ varstore⟦var↦sload evmₛ address⟧) := by
-    aesop
-  apply And.intro
-  rw [← code]
-  exact IsERC20_of_preservesEvm preserves_final is_erc20
+  -- get underlying Preserved from preservesEvm
+  rw [ s_eq_ok, preservesEvm_of_insert, preservesEvm_of_insert ] at preservesEvm
+  have Preserved := Preserved_of_preservesEvm_of_Ok preservesEvm
+
+  -- have : Address.ofUInt256 var_account ∈ erc20.balances := sorry
+  -- obtain ⟨address, hasAddress, hasBalance⟩ := is_erc20.hasBalance this
+  -- obtain ⟨preserves, is_ok, lookup⟩ := keccak hasAddress
+  -- obtain ⟨evmₛ, varstoreₛ, ok_state⟩ := State_of_isOk is_ok
 
   apply And.intro
-  · rw [←code]
-    unfold preservesEvm
-    aesop
-  · rw [← code]
-    have : Ok evmₛ varstore⟦var↦sload evmₛ address⟧[var]!! = sload evmₛ address := by aesop
-    rw [this]
+  -- IsERC20 for the final state
+  exact IsERC20_of_preservesEvm (by aesop) is_erc20
+
+  rw [← code]
+  apply And.intro
+  -- preservesEvm s₀ s₉
+  rw [ preservesEvm_of_insert' ]
+  exact preservesEvm_of_preserved _ _ Preserved
+
+  -- lookup balance
+  clr_varstore
+  by_cases mem : Address.ofUInt256 var_account ∈ erc20.balances
+  -- there is such account in balances
+  obtain ⟨address, has_address, balance⟩ := is_erc20.hasBalance mem
+  have lookup := keccak has_address
+  rw [lookup] at code ⊢
+  rw [ Finmap.mem_lookup_iff (s := erc20.balances), ← Finmap.lookup_eq_some_iff
+     , ← sload_eq_of_preserved Preserved
+     ]
+  have := State.get_evm_of_ok ▸ balance
+  exact this
+
+  -- there is *no* such account in balances
+  rw [this]
     simp
     rw [hasBalance]
     have hPreserved : preserved (Ok evm varstore).evm evmₛ := by
